more progress in insert proof

concurrency/verif_bst_conc_atomic.v
@@ -624,6 +624,7 @@ Proof.
   apply Zle_bool_imp_le in H0. lia.
 Qed.
 
+
 Lemma less_than_irrefl: forall a, less_than a a = false.
 Proof. intros. destruct a; simpl; auto. apply Z.ltb_irrefl. Qed.
 
@@ -923,14 +924,14 @@ Qed.
 
 (* Lemma update_ghost_ref: forall g (tg : @ ghost_tree val)  s g_in, finite s -> (in_tree g lsh1 g_in * ghost_ref g s |-- |==> EX sh1 sh2 g1 g2, ghost_ref g ( Add _ ( Add _ s g1) g2) *
     in_tree g sh1 g1 * in_tree g sh2 g2 * in_tree g lsh1 g_in)%I . *)
-Lemma update_ghost_ref: forall g (tg : @ ghost_tree val)  s g_in, finite s -> (in_tree g g_in * ghost_ref g s |-- |==> EX g1 g2, ghost_ref g ( Add _ ( Add _ s g1) g2) *
+Lemma update_ghost_ref: forall g (tg : @ ghost_tree val)  s g_in  (a: number * number * option ghost_info) (b:number * number * option ghost_info), finite s -> (in_tree g g_in * ghost_ref g s |-- |==> EX g1 g2:gname, both_halves a g1 * both_halves b g2 * ghost_ref g ( Add _ ( Add _ s g1) g2) *
     in_tree g g1 * in_tree g g2 * in_tree g g_in)%I .
  Proof.
  intros.
  iIntros "H".
-iDestruct "H" as "[Ha Hb]". iPoseProof ( in_tree_add with "[$Ha $Hb]") as ">H"; auto.
-iDestruct "H" as ((* sh3 sh4  *)g1) "[[Ha Hb] Hc]". iPoseProof( in_tree_add with "[$Hb $Ha]") as ">Hnew". apply finite_add; auto.
- iDestruct "Hnew" as ((* sh5 sh6 *) g2) "[[Ha Hb ] Hd]". iModIntro. iExists (* sh4, sh6, *) g1, g2. iFrame.
+iDestruct "H" as "[Ha Hb]". iPoseProof ( ghost_node_alloc with "[$Ha $Hb]") as ">H"; auto.
+iDestruct "H" as ((* sh3 sh4  *)g1) "[[[Ha Hb] Hc] Hd]". instantiate(1:= a). iPoseProof( ghost_node_alloc with "[$Hb $Hc]") as ">Hnew". apply finite_add; auto.
+ iDestruct "Hnew" as ((* sh5 sh6 *) g2) "[[[Hc Hb ] He] Hf]". instantiate(1:= b). iModIntro. iExists (* sh4, sh6, *) g1, g2. iFrame.
 Qed.
 
 
@@ -998,18 +999,48 @@ induction tg.
         { simpl. reflexivity. }
 Qed.
 
+Inductive IsEmptyGhostNode (range : number * number * option ghost_info ) :  (@ghost_tree val) -> (number * number) -> Prop :=
+ | InEmptyGhostTree n1 n2 : (range = (n1,n2,@None ghost_info)) -> IsEmptyGhostNode range E_ghost (n1,n2)
+ | InLeftGhostSubTree l g1 x v r g2  n1 n2 : (less_than range.1.2 n2 = true) -> IsEmptyGhostNode range l (n1, Finite_Integer x) -> IsEmptyGhostNode range (T_ghost l g1 x v r g2) (n1,n2) 
+ | InRightGhostSubTree l g1 x v r g2 n1 n2 : (less_than n1 range.1.1 = true) ->  IsEmptyGhostNode range r (Finite_Integer x, n2) -> IsEmptyGhostNode range (T_ghost l g1 x v r g2) (n1,n2).
+ 
+ Lemma range_inside_range_ghost : forall r  r_root tg, IsEmptyGhostNode r tg r_root -> (forall k, In_ghost k tg -> check_key_exist' k r_root = true) -> sorted_ghost_tree tg -> range_inclusion r.1 r_root = true.
+ Proof.
+  intros.
+ revert dependent r_root.
+ induction tg.
+  - intros. inversion H. subst r. apply range_iteself. 
+  - intros. inversion H;subst.
+   * assert ( range_inclusion r.1 (n1, Finite_Integer k) = true ) . 
+       { apply IHtg1 in H10. apply H10. inversion H1;subst. apply H6. inversion H1;subst. unfold gt_ghost in H12.  intros. 
+          assert (check_key_exist' k0 (n1, n2) = true). { apply H0. apply InLeft_ghost. apply H2. } unfold check_key_exist' in *. apply andb_prop in H3. destruct H3. 
+          apply H12 in H2. rewrite H3. assert (less_than (Finite_Integer k0) (Finite_Integer k) = true). { simpl. apply Zaux.Zlt_bool_true. omega. } rewrite H5. auto. } 
+    assert ( check_key_exist' k (n1, n2) = true ) . { apply H0.  apply InRoot_ghost. auto. } unfold check_key_exist' in H3. apply andb_prop in H3. destruct H3.
+    unfold range_inclusion in *. destruct r. destruct p. simpl. apply less_than_to_less_than_equal in H4. apply andb_prop in H2. destruct H2. rewrite H2. 
+    simpl. apply less_than_equal_transitivity with ( b:= Finite_Integer k). apply H5. apply H4. 
+   * assert ( range_inclusion r.1 (Finite_Integer k, n2) = true ) . 
+         { apply IHtg2 in H10. apply H10. inversion H1;subst. apply H11.   inversion H1;subst. unfold lt_ghost in H13.  intros.
+           assert (check_key_exist' k0 (n1, n2) = true). { apply H0. apply InRight_ghost. apply H2. } unfold check_key_exist' in *. apply andb_prop in H3. destruct H3. apply H13 in H2. rewrite H4.
+           assert (less_than (Finite_Integer k) (Finite_Integer k0) = true). { simpl. apply Zaux.Zlt_bool_true. omega. } rewrite H5. auto. }  
+   assert ( check_key_exist' k (n1, n2) = true ) . { apply H0.  apply InRoot_ghost. auto. } unfold check_key_exist' in H3. apply andb_prop in H3. destruct H3.
+   unfold range_inclusion in *. destruct r. destruct p. simpl. apply less_than_to_less_than_equal in H3. apply andb_prop in H2. destruct H2. rewrite H5. 
+  rewrite andb_comm.   simpl. apply less_than_equal_transitivity with ( b:= Finite_Integer k). apply H3. apply H2.
+ Qed.
 
 Lemma extract_public_half_from_ghost_tree_rep_combined:  forall  tg  g_root  g_in x v v0 (r_root: number * number), 
    Ensembles.In gname (find_ghost_set tg g_root) g_in ->(forall k, In_ghost k tg -> check_key_exist' k r_root = true) -> sorted_ghost_tree tg -> ghost_tree_rep tg g_root r_root  |-- EX n:number, EX n0:number, EX o:option ghost_info, !!(range_inclusion (n,n0) r_root = true ) && public_half g_in (n, n0, o) *
-  ( ( ALL g1 g2:gname, ( !!(o = None /\ (check_key_exist' x (n,n0) = true)) &&  public_half g_in (n, n0, Some(x,v,g1,g2)) ) -* ghost_tree_rep (insert_ghost x v tg g1 g2) g_root r_root * my_half g1 (n, Finite_Integer x,@None ghost_info) * my_half g2 (Finite_Integer x, n0, @None ghost_info) )
-  && ( ALL g1 g2:gname, ( !!(o = Some(x,v0,g1,g2) /\ (check_key_exist' x (n,n0) = true)) &&  public_half g_in (n, n0, Some(x,v, g1,g2))) -* ghost_tree_rep (insert_ghost x v tg g1 g2) g_root r_root )
+  ( ( ALL g1 g2:gname, ( !!(o = None /\ (check_key_exist' x (n,n0) = true)) &&  public_half g_in (n, n0, Some(x,v,g1,g2)) * public_half g1 (n, Finite_Integer x,@None ghost_info) * public_half g2 (Finite_Integer x, n0, @None ghost_info) ) -* ( !! IsEmptyGhostNode (n,n0,o) tg r_root && ghost_tree_rep (insert_ghost x v tg g1 g2) g_root r_root  ) )
+  && ( ALL g1 g2:gname, ( !!(o = Some(x,v0,g1,g2) /\ (check_key_exist' x (n,n0) = true)) &&  public_half g_in (n, n0, Some(x,v, g1,g2))) -*  ( !! (~ IsEmptyGhostNode (n,n0,o) tg r_root) && ghost_tree_rep (insert_ghost x v tg g1 g2) g_root r_root ) )
   &&  ( public_half g_in (n, n0, o) -* ghost_tree_rep tg g_root r_root)) .
 Proof.
- (* intros.
+ intros.
 revert dependent r_root.
 revert dependent g_root.
 induction tg.
-  - intros. simpl. simpl in H. inv H. destruct r_root. Exists n n0. Exists (@None ghost_info). entailer!. rewrite less_than_equal_itself. rewrite less_than_equal_itself. auto. repeat apply andp_right. rewrite <- wand_sepcon_adjoint. entailer!. rewrite <- wand_sepcon_adjoint. entailer!. inv H.  apply wand_refl_cancel_right. 
+  - intros. simpl. simpl in H. inv H. destruct r_root. Exists n n0. Exists (@None ghost_info). entailer!. rewrite less_than_equal_itself. rewrite less_than_equal_itself. repeat (split;auto). repeat apply andp_right.
+     { apply allp_right; intro g1. apply allp_right;intro g2. rewrite <- wand_sepcon_adjoint. entailer!. apply InEmptyGhostTree;auto. }
+     { apply allp_right; intro g1. apply allp_right;intro g2. rewrite <- wand_sepcon_adjoint. entailer!. inv H. inv H. }
+     apply wand_refl_cancel_right.  
   - intros. simpl in H. inv H.
     * inv H2.
      { simpl.  destruct r_root. destruct (x <? k) eqn: E1.
@@ -1020,10 +1051,17 @@ induction tg.
         { simpl in H1.  apply andb_prop in H1. destruct H1. assert (check_key_exist' k (n, n0) = true). { apply H0. apply InRoot_ghost. auto. } unfold check_key_exist' in H3.  apply andb_prop in H3. destruct H3. rewrite H1;simpl. apply less_than_to_less_than_equal in H4. apply less_than_equal_transitivity with (b := (Finite_Integer k) ). apply H2. apply H4. }
            rewrite sepcon_assoc. 
         rewrite (sepcon_comm _ (public_half g_root (n, n0, Some (k,v1,g, g0)) *ghost_tree_rep tg2 g0 (Finite_Integer k, n0))). repeat rewrite distrib_sepcon_andp.    repeat apply andp_derives. 
-       {  rewrite (sepcon_comm (public_half g_root (n, n0, Some (k,v1,g, g0))) (ghost_tree_rep (insert_ghost x v tg1 g1 g2) g (n, Finite_Integer k))).
-       rewrite <- (emp_wand (public_half g_root (n, n0, Some (k,v1, g, g0)) *ghost_tree_rep tg2 g0 (Finite_Integer k, n0))) at 1. rewrite wand_sepcon_wand. rewrite emp_sepcon. 
-       rewrite ( sepcon_assoc (ghost_tree_rep (insert_ghost x v tg1 g1 g2) g (n, Finite_Integer k)) _ _). rewrite ( sepcon_comm _ (ghost_tree_rep (insert_ghost x v tg1 g1 g2) g (n, Finite_Integer k)) ). unfold check_key_exist'. simpl less_than. entailer!. }
-       { rewrite <- (emp_wand (public_half g_root (n, n0, Some (k, v1, g, g0)) * ghost_tree_rep tg2 g0 (Finite_Integer k, n0) )). rewrite wand_sepcon_wand. rewrite emp_sepcon. rewrite sepcon_assoc. rewrite (sepcon_comm (ghost_tree_rep tg2 g0 (Finite_Integer k, n0)) _). rewrite <- sepcon_assoc.  unfold check_key_exist'. simpl less_than. entailer!. }
+       { apply allp_right; intro g1. apply allp_right;intro g2.  repeat (rewrite allp_sepcon2; eapply allp_left). instantiate(1:= g2).  instantiate(1:= g1). 
+          rewrite (sepcon_comm (public_half g_root (n, n0, Some (k,v1,g, g0))) (ghost_tree_rep (insert_ghost x v tg1 g1 g2) g (n, Finite_Integer k))).
+          rewrite <- (emp_wand (public_half g_root (n, n0, Some (k,v1, g, g0)) *ghost_tree_rep tg2 g0 (Finite_Integer k, n0))) at 1. rewrite wand_sepcon_wand. rewrite emp_sepcon. 
+         rewrite ( sepcon_assoc (ghost_tree_rep (insert_ghost x v tg1 g1 g2) g (n, Finite_Integer k)) _ _). rewrite ( sepcon_comm (ghost_tree_rep (insert_ghost x v tg1 g1 g2) g (n, Finite_Integer k)) _ ). unfold check_key_exist'. simpl less_than. rewrite <- wand_sepcon_adjoint. rewrite sepcon_comm.  rewrite wand_frame_elim. entailer!. apply InLeftGhostSubTree.
+           { assert (check_key_exist' k (n, n0) = true). { apply H0. apply InRoot_ghost. auto. } unfold check_key_exist' in H3. unfold range_inclusion in H1. apply andb_prop in H1.  apply andb_prop in H3. destruct H1, H3. apply less_than_equal_less_than_transitivity with (b := (Finite_Integer k)).  auto. auto. } apply H2. }
+       { apply allp_right; intro g1. apply allp_right;intro g2. repeat (rewrite allp_sepcon2; eapply allp_left). instantiate(1:= g2).  instantiate(1:= g1).  
+          rewrite <- (emp_wand (public_half g_root (n, n0, Some (k, v1, g, g0)) * ghost_tree_rep tg2 g0 (Finite_Integer k, n0) )). rewrite wand_sepcon_wand. rewrite emp_sepcon. rewrite sepcon_assoc. rewrite (sepcon_comm (ghost_tree_rep tg2 g0 (Finite_Integer k, n0)) _).  rewrite <- sepcon_assoc.  unfold check_key_exist'. simpl less_than.
+          rewrite <- wand_sepcon_adjoint. rewrite sepcon_comm. assert_PROP (check_key_exist' x (n1,n2) = true). { simpl. entailer!. }  rewrite wand_frame_elim. entailer!. inv H4. contradiction H3. apply range_inside_range_ghost in H18. unfold range_inclusion in H18.  apply andb_prop in H18. destruct H18. unfold check_key_exist' in H2.  apply andb_prop in H2. destruct H2.
+          assert (less_than (Finite_Integer k) (Finite_Integer x) = true). { apply less_than_equal_less_than_transitivity with (b:= n1). auto. auto. } simpl in H12. apply Z.ltb_lt in E1. apply Z.ltb_lt in H12. omega. 
+         { intros. assert (check_key_exist' k0 (n, n0) = true). { apply H0. apply InRight_ghost. apply H4. } unfold check_key_exist' in * . apply andb_prop in H5. destruct H5.
+             unfold lt_ghost in H11. apply H11 in H4. rewrite H7;simpl. rewrite andb_comm;simpl.  apply Zaux.Zlt_bool_true. omega. } auto. }
        { rewrite <- ( emp_wand (public_half g_root (n, n0, Some (k,v1,g, g0)) * ghost_tree_rep tg2 g0 (Finite_Integer k, n0))). rewrite wand_sepcon_wand. rewrite emp_sepcon.  rewrite (pull_right _ _ (ghost_tree_rep tg1 g (n, Finite_Integer k))). cancel.  }
       + inv H1. unfold gt_ghost in H10. sep_apply IHtg1. 
       { intros. assert (check_key_exist' k0 (n, n0) = true). { apply H0. apply InLeft_ghost. apply H1. } unfold check_key_exist' in * . apply andb_prop in H2. destruct H2.
@@ -1031,10 +1069,12 @@ induction tg.
       Intros n1 n2 o. Exists n1 n2 o. entailer!.
       { simpl in H1.  apply andb_prop in H1. destruct H1. assert (check_key_exist' k (n, n0) = true). { apply H0. apply InRoot_ghost. auto. } unfold check_key_exist' in H3.  apply andb_prop in H3. destruct H3. rewrite H1;simpl. apply less_than_to_less_than_equal in H4. apply less_than_equal_transitivity with (b := (Finite_Integer k) ). apply H2. apply H4. }
        rewrite sepcon_assoc.  rewrite (sepcon_comm _ (public_half g_root (n, n0, Some (k,v1,g, g0)) *ghost_tree_rep tg2 g0 (Finite_Integer k, n0))). repeat rewrite distrib_sepcon_andp.  repeat  apply andp_derives.
-        { rewrite <- wand_sepcon_adjoint. rewrite sepcon_comm. rewrite <- sepcon_assoc. entailer!. 
+        {  apply allp_right; intro g1. apply allp_right;intro g2. repeat (rewrite allp_sepcon2; eapply allp_left). instantiate(1:= g2).  instantiate(1:= g1).           
+          rewrite <- wand_sepcon_adjoint.  assert_PROP (check_key_exist' x (n1,n2) = true). { simpl. entailer!. } 
           assert (x < k). { simpl in H1. apply andb_prop in H2. apply andb_prop in H1.  destruct H1,H2. unfold less_than_equal, less_than in *. destruct n2.  apply Z.ltb_lt in H4. apply Zle_bool_imp_le in H3. omega. discriminate. discriminate.  } 
           apply Z.ltb_nlt in E1. omega. }
-         { rewrite <- wand_sepcon_adjoint. rewrite sepcon_comm. rewrite <- sepcon_assoc. entailer!. 
+         { apply allp_right; intro g1. apply allp_right;intro g2. repeat (rewrite allp_sepcon2; eapply allp_left). instantiate(1:= g2).  instantiate(1:= g1). 
+          rewrite <- wand_sepcon_adjoint. assert_PROP (check_key_exist' x (n1,n2) = true). { simpl. entailer!. } 
           assert (x < k). { simpl in H1. apply andb_prop in H2. apply andb_prop in H1.  destruct H1,H2. unfold less_than_equal, less_than in *. destruct n2.  apply Z.ltb_lt in H4. apply Zle_bool_imp_le in H3. omega. discriminate. discriminate.  } 
           apply Z.ltb_nlt in E1. omega. }
         { rewrite <- ( emp_wand (public_half g_root (n, n0, Some (k,v1,g, g0)) * ghost_tree_rep tg2 g0 (Finite_Integer k,n0))) at 1. rewrite wand_sepcon_wand. rewrite emp_sepcon. rewrite sepcon_assoc. rewrite (sepcon_comm (ghost_tree_rep tg2 g0 (Finite_Integer k, n0)) _). rewrite sepcon_assoc. cancel.  } 
@@ -1046,11 +1086,13 @@ induction tg.
       Intros n1 n2 o. Exists n1 n2 o. entailer!. 
        { simpl in H1.  apply andb_prop in H1. destruct H1. assert (check_key_exist' k (n, n0) = true). { apply H0. apply InRoot_ghost. auto. } unfold check_key_exist' in H3.  apply andb_prop in H3. destruct H3. rewrite H2;simpl. rewrite andb_comm;simpl. apply less_than_to_less_than_equal in H3. apply less_than_equal_transitivity with (b := (Finite_Integer k) ). apply H3. apply H1. }
        rewrite sepcon_assoc.  rewrite (sepcon_comm _ (public_half g_root (n, n0, Some (k,v1,g, g0)) *ghost_tree_rep tg1 g (n, Finite_Integer k))). repeat rewrite distrib_sepcon_andp.   repeat apply andp_derives.
-        { rewrite <- wand_sepcon_adjoint. rewrite sepcon_comm. rewrite <- sepcon_assoc. entailer!. 
+        { apply allp_right; intro g1. apply allp_right;intro g2. repeat (rewrite allp_sepcon2; eapply allp_left). instantiate(1:= g2).  instantiate(1:= g1). 
+          rewrite <- wand_sepcon_adjoint. assert_PROP (check_key_exist' x (n1,n2) = true). { simpl. entailer!. } 
           assert (k < x). { simpl in H1. apply andb_prop in H2. apply andb_prop in H1.  destruct H1,H2. unfold less_than_equal, less_than in *. destruct n1.  apply Zle_bool_imp_le in H1. apply Z.ltb_lt in H2. omega. discriminate. discriminate.  } 
           apply Z.ltb_lt in E1. omega. }
-          { rewrite <- wand_sepcon_adjoint. rewrite sepcon_comm. rewrite <- sepcon_assoc. entailer!. 
-          assert (k < x). { simpl in H1. apply andb_prop in H2. apply andb_prop in H1.  destruct H1,H2. unfold less_than_equal, less_than in *. destruct n1.  apply Zle_bool_imp_le in H1. apply Z.ltb_lt in H2. omega. discriminate. discriminate.  } 
+          { apply allp_right; intro g1. apply allp_right;intro g2. repeat (rewrite allp_sepcon2; eapply allp_left). instantiate(1:= g2).  instantiate(1:= g1). 
+            rewrite <- wand_sepcon_adjoint. assert_PROP (check_key_exist' x (n1,n2) = true). { simpl. entailer!. }  
+           assert (k < x). { simpl in H1. apply andb_prop in H2. apply andb_prop in H1.  destruct H1,H2. unfold less_than_equal, less_than in *. destruct n1.  apply Zle_bool_imp_le in H1. apply Z.ltb_lt in H2. omega. discriminate. discriminate.  } 
           apply Z.ltb_lt in E1. omega. }
         { rewrite <- ( emp_wand (public_half g_root (n, n0, Some (k,v1,g, g0)) * ghost_tree_rep tg1 g (n,Finite_Integer k))) at 1. rewrite wand_sepcon_wand. rewrite emp_sepcon. rewrite sepcon_assoc. cancel.  } 
 
@@ -1060,12 +1102,18 @@ induction tg.
       Intros n1 n2 o. Exists n1 n2 o. entailer!. 
       { simpl in H1.  apply andb_prop in H1. destruct H1. assert (check_key_exist' k (n, n0) = true). { apply H0. apply InRoot_ghost. auto. } unfold check_key_exist' in H3.  apply andb_prop in H3. destruct H3. rewrite H2;simpl. rewrite andb_comm;simpl.  apply less_than_to_less_than_equal in H3. apply less_than_equal_transitivity with (b := (Finite_Integer k) ). apply H3. apply H1. } 
        rewrite sepcon_assoc. rewrite (sepcon_comm _ (public_half g_root (n, n0, Some (k,v1,g, g0)) *ghost_tree_rep tg1 g (n,Finite_Integer k))). repeat rewrite distrib_sepcon_andp.  repeat apply andp_derives.
-        {  rewrite (sepcon_comm (public_half g_root (n, n0, Some (k,v1,g, g0)) * ghost_tree_rep tg1 g (n, Finite_Integer k)) (ghost_tree_rep (insert_ghost x v tg2 g1 g2) g0 (Finite_Integer k,n0))).
+        { apply allp_right; intro g1. apply allp_right;intro g2. repeat (rewrite allp_sepcon2; eapply allp_left). instantiate(1:= g2).  instantiate(1:= g1).  
+         rewrite (sepcon_comm (public_half g_root (n, n0, Some (k,v1,g, g0)) * ghost_tree_rep tg1 g (n, Finite_Integer k)) (ghost_tree_rep (insert_ghost x v tg2 g1 g2) g0 (Finite_Integer k,n0))).
          rewrite <- (emp_wand (public_half g_root (n, n0, Some (k,v1,g, g0)) *ghost_tree_rep tg1 g (n,Finite_Integer k))) at 1.  rewrite wand_sepcon_wand.  rewrite emp_sepcon. 
-         rewrite ( sepcon_comm _ (ghost_tree_rep (insert_ghost x v tg2 g1 g2) g0 (Finite_Integer k,n0)) ). unfold check_key_exist'. unfold less_than. entailer!. }
-        {  rewrite (sepcon_comm (public_half g_root (n, n0, Some (k,v1,g, g0)) * ghost_tree_rep tg1 g (n, Finite_Integer k)) (ghost_tree_rep (insert_ghost x v tg2 g1 g2) g0 (Finite_Integer k,n0))).
+         unfold check_key_exist'. simpl less_than. rewrite <- wand_sepcon_adjoint. rewrite sepcon_comm.  rewrite wand_frame_elim. entailer!. apply InRightGhostSubTree.
+         { assert (check_key_exist' k (n, n0) = true). { apply H0. apply InRoot_ghost. auto. } unfold check_key_exist' in H3. unfold range_inclusion in H1. apply andb_prop in H1.  apply andb_prop in H3. destruct H1, H3. apply less_than_less_than_equal_transitivity with (b := (Finite_Integer k)).  auto. auto. }   apply H2. } 
+        {  apply allp_right; intro g1. apply allp_right;intro g2. repeat (rewrite allp_sepcon2; eapply allp_left). instantiate(1:= g2).  instantiate(1:= g1). 
+           rewrite (sepcon_comm (public_half g_root (n, n0, Some (k,v1,g, g0)) * ghost_tree_rep tg1 g (n, Finite_Integer k)) (ghost_tree_rep (insert_ghost x v tg2 g1 g2) g0 (Finite_Integer k,n0))).
            rewrite <- (emp_wand (public_half g_root (n, n0, Some (k,v1,g, g0)) *ghost_tree_rep tg1 g (n,Finite_Integer k))) at 1.  rewrite wand_sepcon_wand.  rewrite emp_sepcon. 
-           rewrite ( sepcon_comm _ (ghost_tree_rep (insert_ghost x v tg2 g1 g2) g0 (Finite_Integer k,n0)) ). unfold check_key_exist'. unfold less_than. entailer!. }
+           rewrite <- wand_sepcon_adjoint. rewrite sepcon_comm. assert_PROP (check_key_exist' x (n1,n2) = true). { simpl. entailer!. }  rewrite wand_frame_elim. entailer!. inv H4. contradiction H3. apply range_inside_range_ghost in H18. unfold range_inclusion in H18.  apply andb_prop in H18. destruct H18. unfold check_key_exist' in H2.  apply andb_prop in H2. destruct H2.
+          assert (less_than (Finite_Integer x) (Finite_Integer k) = true). { apply less_than_less_than_equal_transitivity with (b:= n2). auto. auto. } simpl in H12. apply Z.ltb_lt in E2. apply Z.ltb_lt in H12. omega. 
+         { intros. assert (check_key_exist' k0 (n, n0) = true). { apply H0. apply InLeft_ghost. apply H4. } unfold check_key_exist' in * . apply andb_prop in H5. destruct H5.
+             unfold gt_ghost in H10. apply H10 in H4. rewrite H5;simpl.   apply Zaux.Zlt_bool_true. omega. } auto. contradiction H3. }
        { rewrite <- ( emp_wand (public_half g_root (n, n0, Some (k,v1,g, g0)) * ghost_tree_rep tg1 g (n,Finite_Integer k))) at 1. rewrite wand_sepcon_wand. rewrite emp_sepcon. cancel.  }
        inv H1. assert (k = x ). { apply Z.ltb_nlt in E1. apply Z.ltb_nlt in E2. omega. }  sep_apply IHtg2.
          { intros. assert (check_key_exist' k0 (n, n0) = true). { apply H0. apply InRight_ghost. apply H2. } unfold check_key_exist' in * . apply andb_prop in H3. destruct H3.
@@ -1073,31 +1121,29 @@ induction tg.
       Intros n1 n2 o. Exists n1 n2 o. entailer!. 
        { simpl in H2.  apply andb_prop in H2. destruct H2. assert (check_key_exist' x (n, n0) = true). { apply H0. apply InRoot_ghost. auto. } unfold check_key_exist' in H3.  apply andb_prop in H3. destruct H3. rewrite H2;simpl. rewrite andb_comm;simpl. apply less_than_to_less_than_equal in H3. apply less_than_equal_transitivity with (b := (Finite_Integer x) ). apply H3. apply H1. }
        rewrite sepcon_assoc.  rewrite (sepcon_comm _ (public_half g_root (n, n0, Some (x,v1,g, g0)) *ghost_tree_rep tg1 g (n, Finite_Integer x))). repeat rewrite distrib_sepcon_andp.   repeat apply andp_derives.
-        { rewrite <- wand_sepcon_adjoint. rewrite sepcon_comm. rewrite <- sepcon_assoc. entailer!. 
+        { apply allp_right; intro g1. apply allp_right;intro g2. repeat (rewrite allp_sepcon2; eapply allp_left). instantiate(1:= g2).  instantiate(1:= g1).  
+          rewrite <- wand_sepcon_adjoint. assert_PROP (check_key_exist' x (n1,n2) = true). { simpl. entailer!. } 
          simpl in H2.  apply andb_prop in H2. apply andb_prop in H1.  destruct H2, H1. destruct n1. simpl in H1. apply Z.ltb_lt in H1. apply Zle_bool_imp_le in H2. omega. discriminate. simpl in H1. discriminate. }
-        { rewrite <- wand_sepcon_adjoint. rewrite sepcon_comm. rewrite <- sepcon_assoc. entailer!. 
+        { apply allp_right; intro g1. apply allp_right;intro g2. repeat (rewrite allp_sepcon2; eapply allp_left). instantiate(1:= g2).  instantiate(1:= g1). 
+          rewrite <- wand_sepcon_adjoint. assert_PROP (check_key_exist' x (n1,n2) = true). { simpl. entailer!. } 
          simpl in H2.  apply andb_prop in H2. apply andb_prop in H1.  destruct H2, H1. destruct n1. simpl in H1. apply Z.ltb_lt in H1. apply Zle_bool_imp_le in H2. omega. discriminate. simpl in H1. discriminate. }
     
         { rewrite <- ( emp_wand (public_half g_root (n, n0, Some (x,v1,g, g0)) * ghost_tree_rep tg1 g (n,Finite_Integer x))) at 1. rewrite wand_sepcon_wand. rewrite emp_sepcon. rewrite sepcon_assoc. cancel.  } 
      }  
   * inv H2. simpl. destruct r_root. Exists n n0. Exists (Some(k,v1,g,g0)). entailer!. repeat rewrite less_than_equal_itself. simpl;auto. repeat  apply andp_right.
-       { rewrite <- wand_sepcon_adjoint. Intros a. }
-       { rewrite <- wand_sepcon_adjoint. entailer!. inv H. simpl. destruct (x <? x) eqn: E1. apply Z.ltb_lt in E1. omega. simpl. entailer!. }
-       {   rewrite sepcon_assoc. rewrite <- (sepcon_emp (public_half g_in (n, n0, Some (k,v1, g, g0) ))) at 1. rewrite <- wand_sepcon_wand. rewrite emp_wand. cancel. apply wand_refl_cancel_right. }
-  
-Qed. *) 
-Admitted.
+       { apply allp_right; intro g1. apply allp_right;intro g2. rewrite <- wand_sepcon_adjoint. Intros a. }
+       { apply allp_right; intro g1. apply allp_right;intro g2.  rewrite <- wand_sepcon_adjoint. assert_PROP (Some (k, v1, g, g0) = Some (x, v0, g1, g2)). { entailer!. } inv H. simpl. destruct (x <? x) eqn: E1. apply Z.ltb_lt in E1. omega. simpl. entailer!. inv H2. 
+         { simpl in H5. unfold less_than in H5. destruct n0 in H5. apply Z.ltb_lt in H5. omega.  discriminate.  discriminate.   }
+         { simpl in H5. unfold less_than in H5. destruct n in H5. apply Z.ltb_lt in H5. omega.  discriminate.  discriminate. } }
+       {   rewrite sepcon_assoc. rewrite <- (sepcon_emp (public_half g_in (n, n0, Some (k,v1, g, g0) ))) at 1. rewrite <- wand_sepcon_wand. rewrite emp_wand. cancel. apply wand_refl_cancel_right. }  
+Qed. 
 
-Inductive IsEmptyGhostNode (range : number * number ) :  (@ghost_tree val) -> (number * number) -> Prop :=
- | InEmptyGhostTree n1 n2 : (range = (n1,n2)) -> IsEmptyGhostNode range E_ghost (n1,n2)
- | InLeftGhostSubTree l g1 x v r g2  n1 n2 : IsEmptyGhostNode range l (n1, Finite_Integer x) -> IsEmptyGhostNode range (T_ghost l g1 x v r g2) (n1,n2) 
- | InRightGhostSubTree l g1 x v r g2 n1 n2 :  IsEmptyGhostNode range r (Finite_Integer x, n2) -> IsEmptyGhostNode range (T_ghost l g1 x v r g2) (n1,n2).
- 
- Lemma key_not_exist_in_tree: forall  (tg : @ghost_tree val) r_root range x, IsEmptyGhostNode range tg r_root -> check_key_exist' x range = true  -> ~ In_ghost x tg.
+
+ Lemma key_not_exist_in_tree: forall  (tg : @ghost_tree val) r_root range x, IsEmptyGhostNode range tg r_root -> check_key_exist' x range.1 = true  -> ~ In_ghost x tg.
  Proof.
  Admitted.
  
-  Lemma key_exist_in_tree: forall  (tg : @ghost_tree val) r_root range x, ~IsEmptyGhostNode range tg r_root -> check_key_exist' x range = true ->  In_ghost x tg.
+  Lemma key_exist_in_tree: forall  (tg : @ghost_tree val) r_root range x, ~IsEmptyGhostNode range tg r_root -> check_key_exist' x range.1 = true ->  In_ghost x tg.
  Proof.
  Admitted.
  
@@ -1118,11 +1164,11 @@ Qed.
 
 Lemma extract_lemmas_for_treerep2:  forall  t   g g_root  g_in  x v v0,
   sorted_tree t -> tree_rep2 g g_root t * in_tree g g_in |-- EX n, EX n0 ,EX o:option ghost_info, public_half g_in (n, n0, o) *
-  ( (EX g1 g2:gname,( !!(o = None /\ (check_key_exist' x (n,n0) = true)) && public_half g_in (n, n0, Some(x,v,g1,g2)) ) -*   (|==> tree_rep2 g g_root (insert x v t ) * my_half g1 (n, Finite_Integer x,@None ghost_info) * my_half g2 (Finite_Integer x, n0, @None ghost_info) *  in_tree g g_in * in_tree g g1 * in_tree g g2)%I )
-    &&  (ALL g1 g2:gname, ( !!(o = Some(x,v0,g1,g2) /\ (check_key_exist' x (n,n0) = true)) &&  public_half g_in (n, n0, Some(x,v, g1,g2))) -* (|==> tree_rep2 g g_root (insert x v t ) *  in_tree g g_in)%I ) 
+  ( (|==>  (EX g1 g2:gname,( !!(o = None /\ (check_key_exist' x (n,n0) = true)) && public_half g_in (n, n0, Some(x,v,g1,g2)) ) -* tree_rep2 g g_root (insert x v t ) * my_half g1 (n, Finite_Integer x,@None ghost_info) * my_half g2 (Finite_Integer x, n0, @None ghost_info) *  in_tree g g_in * in_tree g g1 * in_tree g g2))%I 
+    &&  (|==>  (ALL g1 g2:gname, ( !!(o = Some(x,v0,g1,g2) /\ (check_key_exist' x (n,n0) = true)) &&  public_half g_in (n, n0, Some(x,v, g1,g2))) -*  tree_rep2 g g_root (insert x v t ) *  in_tree g g_in))%I 
    && ( public_half g_in (n, n0, o) -* (tree_rep2 g g_root t * in_tree g g_in ) )). 
 Proof.
- (* intros.
+  intros.
 unfold tree_rep2 at 1. Intros tg. 
 assert_PROP( Ensembles.In _ (find_ghost_set tg g_root) g_in ). {  rewrite -> sepcon_assoc. rewrite  sepcon_comm.   apply sepcon_derives_prop. rewrite sepcon_comm. apply node_exist_in_tree. }
  rewrite sepcon_assoc. rewrite (sepcon_comm (ghost_ref g (find_ghost_set tg g_root)) _).  rewrite (sepcon_comm (ghost_tree_rep tg g_root (Neg_Infinity, Pos_Infinity)) _).
@@ -1130,30 +1176,24 @@ assert_PROP( Ensembles.In _ (find_ghost_set tg g_root) g_in ). {  rewrite -> sep
   { Intros n1 n2 o.  instantiate (1 := g_in). Exists n1 n2 o.  
  cancel. repeat rewrite ( distrib_sepcon_andp (in_tree g g_in * ghost_ref g (find_ghost_set tg g_root) ) _ _). 
     repeat apply andp_derives.
-     +   assert_PROP ( IsEmptyGhostNode (n1,n2) tg (Neg_Infinity, Pos_Infinity) /\ check_key_exist' x (n1, n2) = true ). { admit. }
-     unfold tree_rep2. iIntros "H". iDestruct "H" as "[[Ha Hb] Hc]". iPoseProof(update_ghost_ref with "[Ha Hb]") as "Hnew". auto.  instantiate(1:= (find_ghost_set tg g_root) ). apply find_ghost_set_finite. iFrame.
-      iMod "Hnew". iDestruct "Hnew" as (g1 g2) "[[[Ha Hb] Hd] H]". 
-       (* rewrite update_ghost_ref. iIntros "(H1 & H2)".  iMod "H1". iDestruct "H1" as (g1 g2) "(((H1 & H3) & H4) & H5)". iModIntro. iExists g1. iExists g2. iIntros "" *)
-      Intros g1 g2. Exists g1 g2.  rewrite <- ( emp_wand (in_tree g g_in * ghost_ref g (find_ghost_set tg g_root) )). rewrite wand_sepcon_wand.  Exists g1 g2.  apply wand_derives. instantiate(1:= v). instantiate(1:=x). entailer!. 
-      iIntros "H". iDestruct "H" as "[[Ha Hb] Hc]". iPoseProof(update_ghost_ref with "[Ha Hb]") as "Hnew".     
-        { instantiate (1 := x).  instantiate(2:=g1). instantiate(1:= g2). instantiate (1 := v). entailer!. } 
-         {  iIntros "H". iDestruct "H" as "[[Ha Hb] Hc]".  normalize. iPoseProof(update_ghost_ref with "[Ha Hb]") as "Hnew". auto. instantiate(1:= (find_ghost_set tg g_root) ). apply find_ghost_set_finite. iFrame. iMod "Hnew".  iExists (insert_ghost x v tg g1 g2). iModIntro. 
-          rewrite ( insert_preserved_in_ghost_tree t tg _ _ _ _). rewrite update_ghost_tree_with_insert.  iFrame. admit. apply (key_not_exist_in_tree tg (Neg_Infinity, Pos_Infinity) (n1,n2) x). destruct H3; auto. destruct H3;auto. auto. } 
-     +   assert_PROP ( ~IsEmptyGhostNode (n1,n2) tg (Neg_Infinity, Pos_Infinity) /\ check_key_exist' x (n1, n2) = true). { admit. }
-
-     unfold tree_rep2.  rewrite <- ( emp_wand (in_tree g g_in * ghost_ref g (find_ghost_set tg g_root) )). rewrite wand_sepcon_wand. apply wand_derives.
-     { entailer!. }
-     { iIntros "H". iDestruct "H" as "[[Ha Hb] Hc]". iModIntro. normalize.   iExists (insert_ghost x v tg g1 g2). rewrite ( insert_preserved_in_ghost_tree t tg _ _ _ _).  rewrite update_ghost_tree_with_insert2. iFrame. iSplit;auto.
-       split.  apply (key_exist_in_tree tg (Neg_Infinity, Pos_Infinity) (n1,n2) x).  destruct H3. apply H3. destruct H3. auto. apply (sortedness_preserved__in_ghosttree t tg). auto. auto. auto. }
-
-    + rewrite <- (emp_wand (in_tree g g_in * ghost_ref g (find_ghost_set tg g_root))). rewrite wand_sepcon_wand. apply wand_derives.
+     +  
+        erewrite update_ghost_ref. iIntros "(H1 & H2)". iMod "H1". iDestruct "H1" as (g1 g2) "(((((H1 & H3) & H4) & H5) & H6) & H7)". instantiate( 9:=  (n1, Finite_Integer x, @None ghost_info) ). instantiate(8:=  (Finite_Integer x, n2, @None ghost_info) ).
+        rewrite <- !both_halves_join. iDestruct "H1" as "(H1 & H1')". iDestruct "H3" as "(H3 & H3')". iModIntro. iExists g1. iExists g2. iIntros "(H & H')". iDestruct "H" as "%".  iSpecialize ("H2" $! g1 g2 ). iSpecialize ("H2" with "[H' H1' H3']"). iFrame. repeat (iSplit;auto).
+        unfold tree_rep2. normalize.  iExists (insert_ghost x v tg g1 g2). rewrite ( insert_preserved_in_ghost_tree t tg _ _ _ _). iDestruct "H2" as "[% H2]". rewrite update_ghost_tree_with_insert. iFrame. repeat (iSplit;auto). 
+        apply (key_not_exist_in_tree tg (Neg_Infinity, Pos_Infinity) (n1,n2,o) x). auto. destruct H3; auto.  auto. auto. apply find_ghost_set_finite.
+     +  
+        iIntros "((H1 & H2) & H3)". iModIntro. iIntros (g1 g2) "[% H]".  iSpecialize ("H3" $! g1 g2 ). iSpecialize ("H3" with "[H]"). iFrame;repeat (iSplit;auto).
+        unfold tree_rep2. normalize.  iExists (insert_ghost x v tg g1 g2). rewrite ( insert_preserved_in_ghost_tree t tg _ _ _ _).  iDestruct "H3" as "[% H3]". rewrite update_ghost_tree_with_insert2. iFrame. repeat (iSplit;auto). split. 
+        apply (key_exist_in_tree tg (Neg_Infinity, Pos_Infinity) (n1,n2,o) x). auto.  destruct H3;auto. apply (sortedness_preserved__in_ghosttree t tg). auto. auto. auto.
+   
+    + rewrite <- (emp_wand (in_tree g g_in * ghost_ref g (find_ghost_set tg g_root))). rewrite wand_sepcon_wand.  apply wand_derives.
        entailer!. unfold tree_rep2. Exists tg. entailer!.
    }
    apply H1. intros. unfold check_key_exist'. simpl. auto.
    { 
      apply (sortedness_preserved__in_ghosttree t tg). auto. auto.   
-   }    *)
-Admitted.
+   }
+Qed.
 
 Definition surely_malloc_spec :=
   DECLARE _surely_malloc
@@ -2117,6 +2157,109 @@ Proof.
   { entailer!. }
 Qed.
 
+  Lemma in_tree_root_range_insert:
+  ∀ (x : Z)(v:val) (g g_root : gname) (Q : mpred) (inv_names : invG)
+    (r : number * number * option ghost_info),
+    (atomic_shift (λ BST : tree, !! sorted_tree BST && tree_rep2 g g_root BST)
+       ∅ ⊤
+       (λ (BST : tree) (_ : ()),
+          !! sorted_tree (insert x v BST) &&
+          tree_rep2 g g_root (insert x v BST) * emp) 
+       (λ _ : (), Q) * my_half g_root r * in_tree g g_root)
+      |-- atomic_shift (λ BST : tree, !! sorted_tree BST && tree_rep2 g g_root BST)
+       ∅ ⊤
+       (λ (BST : tree) (_ : ()),
+          !! sorted_tree (insert x v BST) &&
+          tree_rep2 g g_root (insert x v BST) * emp) 
+       (λ _ : (), Q) * my_half g_root r  * (!! (r.1 = (Neg_Infinity, Pos_Infinity)) && in_tree g g_root).
+Proof.
+  intros. apply sync_rollback. intros t. Intros. unfold tree_rep2 at 1. Intros tg.
+  destruct tg; simpl.
+  - eapply derives_trans; [|apply ghost_seplog.bupd_intro].
+    Exists (Neg_Infinity, Pos_Infinity, @None ghost_info). cancel.
+    apply imp_andp_adjoint. Intros. inv H1. rewrite <- wand_sepcon_adjoint.
+    eapply derives_trans; [|apply ghost_seplog.bupd_intro]. entailer!.
+    unfold tree_rep2. Exists (@E_ghost val). simpl. entailer!.
+  - eapply derives_trans; [|apply ghost_seplog.bupd_intro].
+    Exists (Neg_Infinity, Pos_Infinity, Some (k, v0, g0, g1)). cancel.
+    apply imp_andp_adjoint. Intros. inv H1. rewrite <- wand_sepcon_adjoint.
+    eapply derives_trans; [|apply ghost_seplog.bupd_intro]. entailer!.
+    unfold tree_rep2. Exists (T_ghost tg1 g0 k v0 tg2 g1). simpl. entailer!.
+Qed. 
+
+ Lemma in_tree_left_range_insert:
+  ∀ (x x0: Z) (g g_root : gname) (Q : mpred) (inv_names : invG) (v v0: val)
+    (g_in ga gb: gname) (r a: number * number * option ghost_info),
+    check_key_exist' x r.1 = true -> r.2 = Some (x0, v0, ga, gb) -> x < x0 ->
+    (atomic_shift (λ BST : tree, !! sorted_tree BST && tree_rep2 g g_root BST)  ∅ ⊤
+       (λ (BST : tree) (_ : ()), !! sorted_tree (insert x v BST) &&
+          tree_rep2 g g_root (insert x v BST) * emp) 
+       (λ _ : (), Q)  * my_half g_in r *  in_tree g g_in * my_half ga a)
+    |-- atomic_shift (λ BST : tree, !! sorted_tree BST && tree_rep2 g g_root BST)  ∅ ⊤
+       (λ (BST : tree) (_ : ()), !! sorted_tree (insert x v BST) &&
+          tree_rep2 g g_root (insert x v BST) * emp) 
+       (λ _ : (), Q)  * my_half g_in r * 
+    (!! (a.1 = (r.1.1, Finite_Integer x0)) && (in_tree g g_in * my_half ga a)).
+    
+Proof.
+intros. rewrite sepcon_assoc. apply sync_rollback. intros t.
+  unfold tree_rep2 at 1. Intros tg.
+  assert_PROP (Ensembles.In _ (find_ghost_set tg g_root) g_in). {
+    sep_apply node_exist_in_tree. entailer!. }
+  sep_apply (ghost_tree_rep_public_half_ramif2 _ _ (Neg_Infinity, Pos_Infinity) _ H4).
+  rewrite distrib_orp_sepcon. apply orp_left.
+  - Intros r0. eapply derives_trans; [|apply ghost_seplog.bupd_intro].
+    Exists (r0, @None ghost_info). cancel. apply imp_andp_adjoint. Intros.
+    destruct r as [? rS]. simpl in H0. subst rS. inv H5.
+  - Intros r0 x1 v1 ga0 gb0 i1 i2.
+    eapply derives_trans; [|apply ghost_seplog.bupd_intro].
+    Exists (r0, Some (x1, v1, ga0, gb0)). cancel. apply imp_andp_adjoint. Intros.
+    subst r. simpl fst. simpl in H0. inv H0. simpl in H.
+    assert_PROP (a = (r0.1, Finite_Integer x0, i1)). {
+      sep_apply (@public_agree (number * number * option ghost_info)).
+      entailer!. } destruct a. inv H0. simpl fst.
+    rewrite <- wand_sepcon_adjoint.
+    eapply derives_trans; [|apply ghost_seplog.bupd_intro]. entailer!.
+    unfold tree_rep2. Exists tg. entailer!. rewrite sepcon_comm.
+    rewrite <- !sepcon_assoc. apply wand_frame_elim.
+Qed.
+
+ Lemma in_tree_right_range_insert:
+  ∀ (x x0: Z) (g g_root : gname) (Q : mpred) (inv_names : invG) (v v0: val)
+    (g_in ga gb: gname) (r a: number * number * option ghost_info),
+    check_key_exist' x r.1 = true -> r.2 = Some (x0, v0, ga, gb) -> x0 < x ->
+    atomic_shift (λ BST : tree, !! sorted_tree BST && tree_rep2 g g_root BST)  ∅ ⊤
+       (λ (BST : tree) (_ : ()), !! sorted_tree (insert x v BST) &&
+          tree_rep2 g g_root (insert x v BST) * emp) 
+       (λ _ : (), Q)  * my_half g_in r *  in_tree g g_in * my_half gb a
+    |-- atomic_shift (λ BST : tree, !! sorted_tree BST && tree_rep2 g g_root BST)  ∅ ⊤
+       (λ (BST : tree) (_ : ()), !! sorted_tree (insert x v BST) &&
+          tree_rep2 g g_root (insert x v BST) * emp) 
+       (λ _ : (), Q)  * my_half g_in r * 
+    (!! (a.1 = ( Finite_Integer x0, r.1.2)) && (in_tree g g_in * my_half gb a)).
+    
+Proof.
+intros. rewrite sepcon_assoc. apply sync_rollback. intros t.
+  unfold tree_rep2 at 1. Intros tg.
+  assert_PROP (Ensembles.In _ (find_ghost_set tg g_root) g_in). {
+    sep_apply node_exist_in_tree. entailer!. }
+  sep_apply (ghost_tree_rep_public_half_ramif2 _ _ (Neg_Infinity, Pos_Infinity) _ H4).
+  rewrite distrib_orp_sepcon. apply orp_left.
+  - Intros r0. eapply derives_trans; [|apply ghost_seplog.bupd_intro].
+    Exists (r0, @None ghost_info). cancel. apply imp_andp_adjoint. Intros.
+    destruct r as [? rS]. simpl in H0. subst rS. inv H5.
+  - Intros r0 x1 v1 ga0 gb0 i1 i2.
+    eapply derives_trans; [|apply ghost_seplog.bupd_intro].
+    Exists (r0, Some (x1, v1, ga0, gb0)). cancel. apply imp_andp_adjoint. Intros.
+    subst r. simpl fst. simpl in H0. inv H0. simpl in H.
+    assert_PROP (a = (Finite_Integer x0, r0.2, i2)). {
+      sep_apply (@public_agree (number * number * option ghost_info)).
+      entailer!. } destruct a. inv H0. simpl fst.
+    rewrite <- wand_sepcon_adjoint.
+    eapply derives_trans; [|apply ghost_seplog.bupd_intro]. entailer!.
+    unfold tree_rep2. Exists tg. entailer!. rewrite sepcon_comm.
+    rewrite <- !sepcon_assoc. apply wand_frame_elim.
+Qed.
 
 Lemma body_insert: semax_body Vprog Gprog f_insert insert_spec.
 Proof.
@@ -2131,7 +2274,9 @@ Proof.
   * (* Precondition *)
     unfold insert_inv.
     unfold node_lock_inv at 2. rewrite selflock_eq. unfold node_lock_inv_pred at 1. unfold sync_inv at 1. unfold nodebox_rep, ltree. Intro r. Exists r g_root lock np. Exists np.
-     unfold node_lock_inv. entailer!. admit. 
+    rewrite node_rep_def. Intros tp. gather_SEP (atomic_shift _ _ _ _ _) (my_half _ _) (in_tree g _ ).  
+    sep_apply ( in_tree_root_range_insert x v g g_root Q inv_names r).
+     unfold node_lock_inv. Exists tp. entailer!. rewrite H11. simpl. auto. 
   * (* Loop body *)
     unfold insert_inv.
     Intros  r g_in lock_in np0.
@@ -2168,10 +2313,10 @@ Proof.
             eapply sync_commit_gen1.
             intros. iIntros "H". iDestruct "H" as "[H1 H2]". iDestruct "H2" as "[% H2]".
              iModIntro.  iPoseProof ( extract_lemmas_for_treerep2 with "[H1 H2]") as "Hadd". instantiate(1:= x0 ). auto. iFrame. iDestruct "Hadd" as (n1 n2 o0) "(H1 & H2)". 
-             iExists (n1,n2,o0). iFrame. iPoseProof ( bi.and_elim_l with "H2") as "H3".  iPoseProof ( bi.and_elim_l with "H3") as "Hnew". iIntros "%". iDestruct "Hnew" as (g1 g2) "H".  iExists (n1,n2,Some(x,v,g1,g2)).  iIntros "(H1 & H2)".
-             match goal with |-context[(|==> ?P)%logic] => change ((|==> P)%logic) with ((|==> P)%I) end. instantiate (1 := x). instantiate (1:= v). inv a.  iSpecialize ("H" with "[H2]"). iFrame. iSplit;auto. iMod "H". iModIntro. normalize. 
+             iExists (n1,n2,o0). iFrame. iPoseProof ( bi.and_elim_l with "H2") as "H3".  iPoseProof ( bi.and_elim_l with "H3") as "Hnew". iIntros "%". iMod "Hnew".   iDestruct "Hnew" as (g1 g2) "H". iAlways.  iExists (n1,n2,Some(x,v,g1,g2)).  iIntros "(H1 & H2)".
+             match goal with |-context[(|==> ?P)%logic] => change ((|==> P)%logic) with ((|==> P)%I) end. instantiate (1 := x). instantiate (1:= v).  inv a.  iSpecialize ("H" with "[H2]"). iFrame. iSplit;auto. iModIntro. normalize. 
              iExists g1. normalize.  iExists g2. iDestruct "H" as "(((((H2 & H3) & H4) & H5) & H6) & H7 )". apply (insert_sorted x v) in H7.  iFrame.  iSplit.  auto. auto. done.
-       }
+        }
       Intros g1 g2.
       forward_call (l1, Ews, (node_lock_inv g p1' g1 l1)).
       Intros.
@@ -2222,15 +2367,17 @@ Proof.
         forward.
         forward_call (locka, lsh1,(node_lock_inv g pa ga locka)).
         Intros .
+        unfold node_lock_inv at 2. rewrite selflock_eq. unfold node_lock_inv_pred at 1.  unfold sync_inv at 1.  Intros a.
+         rewrite node_rep_def. Intros tp1. gather_SEP (atomic_shift _ _ _ _ _) (my_half g_in _) (in_tree g g_in) (my_half ga a). 
+         sep_apply (in_tree_left_range_insert x x0 g g_root Q inv_names v v0 g_in ga gb r a). Intros.
         forward_call(lock_in, lsh2, (node_lock_inv_pred g np0 g_in lock_in) ,(node_lock_inv g np0 g_in lock_in)).
         { lock_props.
-          unfold node_lock_inv at 4.  rewrite selflock_eq . unfold node_lock_inv_pred at 1.  unfold sync_inv at 1. Exists r. 
-          rewrite node_rep_def. Exists tp.  cancel. unfold tree_rep_R. rewrite if_false.  assert_PROP (tp <> nullval). { entailer!. }  
+          unfold node_lock_inv at 3. change (selflock (node_lock_inv_pred g pa ga locka) lsh2 locka) with (node_lock_inv g pa ga locka). rewrite selflock_eq . unfold node_lock_inv_pred at 1.  unfold sync_inv at 1. Exists r. 
+          rewrite node_rep_def. Exists tp.  cancel. unfold tree_rep_R at 2. rewrite if_false.  assert_PROP (tp <> nullval). { entailer!. } 
           Exists ga gb x0 v0 pa pb locka lockb.  unfold ltree at 2. entailer!.   repeat rewrite later_sepcon. unfold node_lock_inv at 3. unfold_data_at (data_at _ _ _ tp); entailer!. auto. 
-           }
-          unfold node_lock_inv at 1. rewrite selflock_eq. unfold node_lock_inv_pred at 1.  unfold sync_inv at 1. Intros a.
-         Exists a ga locka pa. unfold node_lock_inv.
-         entailer!. admit.
+        }
+         Exists a ga locka pa. unfold node_lock_inv. rewrite node_rep_def. Exists tp1. 
+         entailer!. rewrite H11. destruct r,p. simpl. unfold check_key_exist' in H3.  apply andb_prop in H3;destruct H3. rewrite H3;simpl. apply Zaux.Zlt_bool_true;auto.
       - (* Inner if, second branch:  k<x *)
         forward. 
         forward.
@@ -2239,15 +2386,17 @@ Proof.
         forward.
         forward_call (lockb, lsh1,(node_lock_inv g pb gb lockb)).
         Intros .
+        unfold node_lock_inv at 2. rewrite selflock_eq. unfold node_lock_inv_pred at 1.  unfold sync_inv at 1.  Intros a.
+        rewrite node_rep_def. Intros tp1. gather_SEP (atomic_shift _ _ _ _ _) (my_half g_in _) (in_tree g g_in) (my_half gb a). 
+        sep_apply (in_tree_right_range_insert x x0 g g_root Q inv_names v v0 g_in ga gb r a). Intros.     
         forward_call(lock_in, lsh2, (node_lock_inv_pred g np0 g_in lock_in) ,(node_lock_inv g np0 g_in lock_in)).
         { lock_props.
-          unfold node_lock_inv at 4.  rewrite selflock_eq . unfold node_lock_inv_pred at 1.  unfold sync_inv at 1. Exists r. 
-          rewrite node_rep_def. Exists tp.  cancel. unfold tree_rep_R. rewrite if_false.  assert_PROP (tp <> nullval). { entailer!. }  
+          unfold node_lock_inv at 3. change (selflock (node_lock_inv_pred g pb gb lockb) lsh2 lockb) with (node_lock_inv g pb gb lockb).   rewrite selflock_eq . unfold node_lock_inv_pred at 1.  unfold sync_inv at 1. Exists r. 
+          rewrite node_rep_def. Exists tp.  cancel. unfold tree_rep_R at 2. rewrite if_false.  assert_PROP (tp <> nullval). { entailer!. }  
           Exists ga gb x0 v0 pa pb locka lockb.  unfold ltree at 3. entailer!.   repeat rewrite later_sepcon. unfold node_lock_inv at 3. unfold_data_at (data_at _ _ _ tp); entailer!. auto. 
          }
-         unfold node_lock_inv at 1. rewrite selflock_eq. unfold node_lock_inv_pred at 1.  unfold sync_inv at 1. Intros a.
-         Exists a gb lockb pb. unfold node_lock_inv.
-         entailer!. admit.
+         Exists a gb lockb pb. unfold node_lock_inv. rewrite node_rep_def. Exists tp1. 
+         entailer!. rewrite H12. destruct r,p.  unfold check_key_exist' in H3.  apply andb_prop in H3;destruct H3. unfold check_key_exist'. rewrite H19;simpl. rewrite andb_comm. apply Zaux.Zlt_bool_true;auto.
       - (* x = k *)
         forward.
         destruct r. destruct p. destruct o. destruct g0. simpl in H5. destruct p.
@@ -2259,9 +2408,9 @@ Proof.
           go_lower.   eapply sync_commit_gen1.
           intros. iIntros "H". iDestruct "H" as "[H1 H2]". iDestruct "H2" as "[% H2]".
           iModIntro.  iPoseProof ( extract_lemmas_for_treerep2 with "[H1 H2]") as "Hadd". instantiate(1:= x1 ). auto. iFrame. iDestruct "Hadd" as (n1 n2 o0) "(H1 & H2)". 
-          iExists (n1,n2,o0). iFrame. iPoseProof ( bi.and_elim_l with "H2") as "H3".  iPoseProof ( bi.and_elim_r with "H3") as "Hnew".  iIntros "%". iSpecialize ("Hnew" $! ga gb).  iExists (n1,n2,Some(x,v,ga,gb)). 
+          iExists (n1,n2,o0). iFrame. iPoseProof ( bi.and_elim_l with "H2") as "H3".  iPoseProof ( bi.and_elim_r with "H3") as "Hnew".  iIntros "%".  iMod "Hnew". iSpecialize ("Hnew" $! ga gb). iAlways.  iExists (n1,n2,Some(x,v,ga,gb)). 
           match goal with |-context[(|==> ?P)%logic] => change ((|==> P)%logic) with ((|==> P)%I) end. instantiate (1 := v). instantiate (1:= x). instantiate (1:= v0). inv a.  iIntros "(H1 & H2)".  iSpecialize ("Hnew" with "[H2]"). inv H5.  
-           iFrame.  iSplit. iSplit. auto. auto. auto.   iMod "Hnew". iModIntro. normalize. iDestruct "Hnew" as "(H2 & H3)". apply (insert_sorted x0 v) in H13. iFrame.  iSplit.  auto. auto. done.
+           iFrame.  iSplit. iSplit. auto. auto. auto.  iModIntro. normalize. iDestruct "Hnew" as "(H2 & H3)". apply (insert_sorted x0 v) in H13. iFrame.  iSplit.  auto. auto. done.
         }
         forward_call(lock_in, lsh2, (node_lock_inv_pred g np0 g_in lock_in) ,(node_lock_inv g np0 g_in lock_in)).
         { lock_props.
@@ -2271,8 +2420,8 @@ Proof.
         forward. entailer!. simpl in H5. discriminate.
        - auto.
   * (* After the loop *)
-    forward. normalize.
-Admitted.
+    forward. normalize. 
+Qed.
 
 
 (* Program Definition lookup_spec :=
